System.v
@@ -6,6 +6,6 @@ a template for system models, capturing common elements of all such
 models, as needed by our overall framework.
 *)
 
-Class System (Stakeholder Resource Phase Context Model: Set) := {}.
+Class System (Stakeholder Resource Phase Context StateModel: Set) := {}.
 
 
